Updated sample computations with oalists

OAlist/Buchberger_Examples.thy
@@ -6,25 +6,21 @@ theory Buchberger_Examples
   imports "../Groebner_Bases/Buchberger" "Algorithm_Schema_Impl" "../Print" "../Groebner_Bases/Code_Target_Rat"
 begin
 
-lemma greater_eq_of_comp: "greater_eq_of_comp = drlex_pm"
-  by (rule, rule, simp add: c.less_eq_of_comparator_def compare_poly_mapping_def drlex_pm_refl)
+subsection \<open>Scalar Polynomials\<close>
 
-lemma greater_of_comp: "greater_of_comp = drlex_pm_strict"
-  apply (rule, rule, simp add: c.less_of_comparator_def compare_poly_mapping_def drlex_pm_strict_def)
-  using drlex_pm_antisym by blast
-
-global_interpretation punit': gd_powerprod drlex_pm "drlex_pm_strict::(('a::{countable,compare,wellorder} \<Rightarrow>\<^sub>0 'b::add_wellorder) \<Rightarrow> _)"
+global_interpretation punit': gd_powerprod "ord_pp_punit cmp_term" "ord_pp_strict_punit cmp_term"
   rewrites "punit.adds_term = (adds)"
-  and "punit.pp_of_term = id"
+  and "punit.pp_of_term = (\<lambda>x. x)"
   and "punit.component_of_term = (\<lambda>_. ())"
   and "punit.monom_mult = monom_mult_punit"
   and "punit.mult_scalar = mult_scalar_punit"
   and "punit'.punit.min_term = min_term_punit"
-  and "punit'.punit.lt = lt_punit"
-  and "punit'.punit.lc = lc_punit"
-  and "punit'.punit.tail = tail_punit"
-  and "punit'.punit.ord_p = ord_p_punit"
-  and "punit'.punit.ord_strict_p = ord_strict_p_punit"
+  and "punit'.punit.lt = lt_punit cmp_term"
+  and "punit'.punit.lc = lc_punit cmp_term"
+  and "punit'.punit.tail = tail_punit cmp_term"
+  and "punit'.punit.ord_p = ord_p_punit cmp_term"
+  and "punit'.punit.ord_strict_p = ord_strict_p_punit cmp_term"
+  for cmp_term :: "('a::nat, 'b::{nat,add_wellorder}) pp nat_term_order"
 
   defines find_adds_punit = punit'.punit.find_adds
   and trd_aux_punit = punit'.punit.trd_aux
@@ -51,74 +47,61 @@ global_interpretation punit': gd_powerprod drlex_pm "drlex_pm_strict::(('a::{cou
   and gb_red_punit = punit'.punit.gb_red
   and gb_aux_punit = punit'.punit.gb_aux_punit
   and gb_punit = punit'.punit.gb_punit \<comment>\<open>Faster, because incorporates product criterion.\<close>
-proof -
-  show "gd_powerprod drlex_pm drlex_pm_strict"
-    apply standard
-    subgoal by (simp add: drlex_pm_strict_def)
-    subgoal by (rule drlex_pm_refl)
-    subgoal by (erule drlex_pm_trans, simp)
-    subgoal by (erule drlex_pm_antisym, simp)
-    subgoal by (rule drlex_pm_lin)
-    subgoal by (rule drlex_pm_zero_min)
-    subgoal by (erule drlex_pm_plus_monotone)
-    done
-  show "punit.adds_term = (adds)" by (fact punit_adds_term)
-  show "punit.pp_of_term = id" by (fact punit_pp_of_term)
-  show "punit.component_of_term = (\<lambda>_. ())" by (fact punit_component_of_term)
-  show "punit.monom_mult = monom_mult_punit" by (simp only: monom_mult_punit_def)
-  show "punit.mult_scalar = mult_scalar_punit" by (simp only: mult_scalar_punit_def)
-qed (simp_all only: min_term_punit_def lt_punit_def lc_punit_def tail_punit_def ord_p_punit_def
-    ord_strict_p_punit_def greater_eq_of_comp greater_of_comp)
-
-lemmas [code_unfold] = id_def
-
-consts pm_to_list :: "('a \<Rightarrow>\<^sub>0 'b) \<Rightarrow> ('a \<times> 'b) list"
-
-lemma compute_pm_to_list [code]: "pm_to_list (Pm_oalist xs) = list_of_oalist xs"
-  sorry
+  subgoal by (fact gd_powerprod_ord_pp_punit)
+  subgoal by (fact punit_adds_term)
+  subgoal by (simp add: id_def)
+  subgoal by (fact punit_component_of_term)
+  subgoal by (simp only: monom_mult_punit_def)
+  subgoal by (simp only: mult_scalar_punit_def)
+  subgoal using min_term_punit_def by fastforce
+  subgoal by (simp only: lt_punit_def ord_pp_punit_alt)
+  subgoal by (simp only: lc_punit_def ord_pp_punit_alt)
+  subgoal by (simp only: tail_punit_def ord_pp_punit_alt)
+  subgoal by (simp only: ord_p_punit_def ord_pp_strict_punit_alt)
+  subgoal by (simp only: ord_strict_p_punit_def ord_pp_strict_punit_alt)
+  done
 
 lemma compute_spoly_punit [code]:
-  "spoly_punit p q = (let t1 = lt_punit p; t2 = lt_punit q; l = lcs t1 t2 in
-         (monom_mult_punit (1 / lc_punit p) (l - t1) p) - (monom_mult_punit (1 / lc_punit q) (l - t2) q))"
-  sorry
+  "spoly_punit to p q = (let t1 = lt_punit to p; t2 = lt_punit to q; l = lcs t1 t2 in
+         (monom_mult_punit (1 / lc_punit to p) (l - t1) p) - (monom_mult_punit (1 / lc_punit to q) (l - t2) q))"
+  by (simp add: punit'.punit.spoly_def Let_def punit'.punit.lc_def)
 
 lemma compute_trd_aux_punit [code]:
-  "trd_aux_punit fs p r =
+  "trd_aux_punit to fs p r =
     (if is_zero p then
       r
     else
-      case find_adds_punit fs (lt_punit p) of
-        None   \<Rightarrow> trd_aux_punit fs (tail_punit p) (plus_monomial_less r (lc_punit p) (lt_punit p))
-      | Some f \<Rightarrow> trd_aux_punit fs (tail_punit p - monom_mult_punit (lc_punit p / lc_punit f) (lt_punit p - lt_punit f) (tail_punit f)) r
+      case find_adds_punit to fs (lt_punit to p) of
+        None   \<Rightarrow> trd_aux_punit to fs (tail_punit to p) (plus_monomial_less r (lc_punit to p) (lt_punit to p))
+      | Some f \<Rightarrow> trd_aux_punit to fs (tail_punit to p - monom_mult_punit (lc_punit to p / lc_punit to f) (lt_punit to p - lt_punit to f) (tail_punit to f)) r
     )"
-  apply (simp only: trd_aux_punit_def)
-  sorry
+  by (simp only: punit'.punit.trd_aux.simps[of to fs p r] plus_monomial_less_def is_zero_def)
 
 function trd_aux_punit_print where
-  "trd_aux_punit_print fs p r (i::nat) (j::nat) =
+  "trd_aux_punit_print to fs p r (i::nat) (j::nat) =
     (if is_zero p then
       print (i, j) r
     else
-      case find_adds_punit fs (lt_punit p) of
-        None   \<Rightarrow> trd_aux_punit_print fs (tail_punit p) (plus_monomial_less r (lc_punit p) (lt_punit p)) (Suc i) j
-      | Some f \<Rightarrow> trd_aux_punit_print fs
-                    (timing (tail_punit p - monom_mult_punit (lc_punit p / lc_punit f) (lt_punit p - lt_punit f) (tail_punit f)))
-                    (print (lc_punit p / lc_punit f) r)
+      case find_adds_punit to fs (lt_punit to p) of
+        None   \<Rightarrow> trd_aux_punit_print to fs (tail_punit to p) (plus_monomial_less r (lc_punit to p) (lt_punit to p)) (Suc i) j
+      | Some f \<Rightarrow> trd_aux_punit_print to fs
+                    (timing (tail_punit to p - monom_mult_punit (lc_punit to p / lc_punit to f) (lt_punit to p - lt_punit to f) (tail_punit to f)))
+                    (print (lc_punit to p / lc_punit to f) r)
                     i (Suc j)
     )"
   by auto
 termination sorry
 
-definition "product_crit_punit_print =
-  (\<lambda>gs bs ps data p q. if product_crit_punit gs bs ps data p q then (print ''prod'' True) else False)"
+definition "product_crit_punit_print to =
+  (\<lambda>gs bs ps data p q. if product_crit_punit to gs bs ps data p q then (print ''prod'' True) else False)"
 
-definition "chain_ncrit_punit_print =
-  (\<lambda>data gs bs hs ps q_in_bs p q. if chain_ncrit_punit data gs bs hs ps q_in_bs p q then (print ''nchain'' True) else False)"
+definition "chain_ncrit_punit_print to =
+  (\<lambda>data gs bs hs ps q_in_bs p q. if chain_ncrit_punit to data gs bs hs ps q_in_bs p q then (print ''nchain'' True) else False)"
 
-definition "chain_ocrit_punit_print =
-  (\<lambda>data hs ps p q. if chain_ocrit_punit data hs ps p q then (print ''ochain'' True) else False)"
+definition "chain_ocrit_punit_print to =
+  (\<lambda>data hs ps p q. if chain_ocrit_punit to data hs ps p q then (print ''ochain'' True) else False)"
 
-definition "trdsp_punit_timing = (\<lambda>bs p. timing_lbl ''trdsp'' (trd_punit bs (spoly_punit (fst (fst p)) (fst (snd p)))))"
+definition "trdsp_punit_timing to = (\<lambda>bs p. timing_lbl ''trdsp'' (trd_punit to bs (spoly_punit to (fst (fst p)) (fst (snd p)))))"
 
 definition "add_pairs_punit_timing =
   (\<lambda>np icrit ncrit ocrit comb gs bs ps hs data.
@@ -135,9 +118,6 @@ definition "add_pairs_punit_print =
 definition "add_basis_sorted_print =
   (\<lambda>rel gs bs ns data. (if length ns = 0 then (\<lambda>_ x. x) else print) (length bs + length ns, map (card_keys \<circ> fst) ns) (merge_wrt (rel data) bs ns))"
 
-definition "add_basis_sorted_print2 =
-  (\<lambda>rel gs bs ns data. print (length (filter (\<lambda>b. let v = lt_punit (fst b) in \<exists>h\<in>set ns. adds_pm_add_linorder (lt_punit (fst h)) v) bs)) (merge_wrt (rel data) bs ns))"
-
 definition "add_basis_sorted_timing =
   (\<lambda>rel gs bs ns data. timing_lbl ''ab'' (merge_wrt (rel data) bs ns))"
 
@@ -145,13 +125,13 @@ definition "gb_sel_punit_print =
   (\<lambda>_ _ ps _. print (length ps) (if List.null ps then [] else [hd ps]))"
 
 lemma product_crit_punit_print [simp]: "product_crit_punit_print = product_crit_punit"
-  by (simp add: product_crit_punit_print_def)
+  by (rule ext, simp add: product_crit_punit_print_def)
 
 lemma chain_ncrit_punit_print [simp]: "chain_ncrit_punit_print = chain_ncrit_punit"
-  by (simp add: chain_ncrit_punit_print_def)
+  by (rule ext, simp add: chain_ncrit_punit_print_def)
 
 lemma chain_ocrit_punit_print [simp]: "chain_ocrit_punit_print = chain_ocrit_punit"
-  by (simp add: chain_ocrit_punit_print_def)
+  by (rule ext, simp add: chain_ocrit_punit_print_def)
 
 (*
 lemma pc_crit_punit_print [code_abbrev]: "pc_crit_punit_print = pc_crit_punit"
@@ -209,47 +189,49 @@ experiment begin interpretation trivariate\<^sub>0_rat .
 subsubsection \<open>Computations\<close>
 
 lemma
-  "lt_punit (X\<^sup>2 * Z ^ 3 + 3 * X\<^sup>2 * Y) = sparse\<^sub>0 [(0, 2), (2, 3)]"
+  "lt_punit DRLEX (X\<^sup>2 * Z ^ 3 + 3 * X\<^sup>2 * Y) = sparse\<^sub>0 [(0, 2), (2, 3)]"
   by eval
 
 lemma
-  "lc_punit (X\<^sup>2 * Z ^ 3 + 3 * X\<^sup>2 * Y) = 1"
+  "lc_punit DRLEX (X\<^sup>2 * Z ^ 3 + 3 * X\<^sup>2 * Y) = 1"
   by eval
 
 lemma
-  "tail_punit (X\<^sup>2 * Z ^ 3 + 3 * X\<^sup>2 * Y) = 3 * X\<^sup>2 * Y"
+  "tail_punit DRLEX (X\<^sup>2 * Z ^ 3 + 3 * X\<^sup>2 * Y) = 3 * X\<^sup>2 * Y"
   by eval
 
 lemma
-  "ord_strict_p_punit (X\<^sup>2 * Z ^ 4 - 2 * Y ^ 3 * Z\<^sup>2) (X\<^sup>2 * Z ^ 7 + 2 * Y ^ 3 * Z\<^sup>2)"
+  "ord_strict_p_punit DRLEX (X\<^sup>2 * Z ^ 4 - 2 * Y ^ 3 * Z\<^sup>2) (X\<^sup>2 * Z ^ 7 + 2 * Y ^ 3 * Z\<^sup>2)"
   by eval
 
+value [code] "(sparse\<^sub>0 [(0::nat, 2::nat), (2, 1)]) adds (sparse\<^sub>0 [(0, 3), (1, 2), (2, 1)])"
+
 lemma
-  "trd_punit [Y\<^sup>2 * Z + 2 * Y * Z ^ 3] (X\<^sup>2 * Z ^ 4 - 2 * Y ^ 3 * Z ^ 3) =
+  "trd_punit DRLEX [Y\<^sup>2 * Z + 2 * Y * Z ^ 3] (X\<^sup>2 * Z ^ 4 - 2 * Y ^ 3 * Z ^ 3) =
     X\<^sup>2 * Z ^ 4 + Y ^ 4 * Z"
   by eval
 
 lemma
-  "spoly_punit (X\<^sup>2 * Z ^ 4 - 2 * Y ^ 3 * Z\<^sup>2) (Y\<^sup>2 * Z + 2 * Z ^ 3) =
-    -2 * Y ^ 3 * Z\<^sup>2 - (Const\<^sub>0 (1 / 2)) * X\<^sup>2 * Y\<^sup>2 * Z\<^sup>2"
+  "spoly_punit DRLEX (X\<^sup>2 * Z ^ 4 - 2 * Y ^ 3 * Z\<^sup>2) (Y\<^sup>2 * Z + 2 * Z ^ 3) =
+    -2 * Y ^ 3 * Z\<^sup>2 - (C\<^sub>0 (1 / 2)) * X\<^sup>2 * Y\<^sup>2 * Z\<^sup>2"
   by eval
 
 lemma
-  "gb_punit
+  "gb_punit DRLEX
     [
      (X\<^sup>2 * Z ^ 4 - 2 * Y ^ 3 * Z\<^sup>2, ()),
      (Y\<^sup>2 * Z + 2 * Z ^ 3, ())
     ] () =
     [
-     (-2 * Y ^ 3 * Z\<^sup>2 - (Const\<^sub>0 (1 / 2)) * X\<^sup>2 * Y\<^sup>2 * Z\<^sup>2, ()),
+     (-2 * Y ^ 3 * Z\<^sup>2 - (C\<^sub>0 (1 / 2)) * X\<^sup>2 * Y\<^sup>2 * Z\<^sup>2, ()),
      (X\<^sup>2 * Z ^ 4 - 2 * Y ^ 3 * Z\<^sup>2, ()),
      (Y\<^sup>2 * Z + 2 * Z ^ 3, ()),
-     (- (Const\<^sub>0 (1 / 2)) * X\<^sup>2 * Y ^ 4 * Z - 2 * Y ^ 5 * Z, ())
+     (- (C\<^sub>0 (1 / 2)) * X\<^sup>2 * Y ^ 4 * Z - 2 * Y ^ 5 * Z, ())
     ]"
   by eval
 
 lemma
-  "gb_punit
+  "gb_punit DRLEX
     [
      (X\<^sup>2 * Z\<^sup>2 - Y, ()),
      (Y\<^sup>2 * Z - 1, ())
@@ -262,7 +244,7 @@ lemma
   by eval
 
 lemma
-  "gb_punit
+  "gb_punit DRLEX
     [
      (X ^ 3 - X * Y * Z\<^sup>2, ()),
      (Y\<^sup>2 * Z - 1, ())
@@ -276,7 +258,7 @@ lemma
   by eval
 
 lemma
-  "gb_punit
+  "gb_punit DRLEX
     [
      (X\<^sup>2 + Y\<^sup>2 + Z\<^sup>2 - 1, ()),
      (X * Y - Z - 1, ()),
@@ -290,11 +272,11 @@ lemma
 
 end
 
-definition "gb_cyclic n = (gb_punit (map (\<lambda>p. (p, ())) (rev ((cyclic n)::(_ \<Rightarrow>\<^sub>0 rat) list))) ())"
+definition "gb_cyclic to n = (gb_punit to (map (\<lambda>p. (p, ())) (rev ((cyclic to n)::(_ \<Rightarrow>\<^sub>0 rat) list))) ())"
 
-value [code] "timing (length (gb_punit (map (\<lambda>p. (p, ())) (Katsura 2)) ()))"
+value [code] "timing (length (gb_punit DRLEX (map (\<lambda>p. (p, ())) (Katsura DRLEX 2)) ()))"
 
-value [code] "timing (length (gb_cyclic 5))"
+value [code] "timing (length (gb_cyclic DRLEX 5))"
 
 function repeat :: "(natural \<Rightarrow> 'c) \<Rightarrow> natural \<Rightarrow> 'c" where
   "repeat f n = (if n = 0 then f 0 else (let _ = f n in repeat f (n - 1)))"
@@ -307,5 +289,151 @@ value [code] "let r1 = (1587403220023648961010354787510025/754422498806579781314
 
 (* The same computation takes 0.004 seconds with Ratio.ratio in OCaml!
   The denominator of r2 with 200+ digits actually appears in the computation of cyclic-6. *)
+
+subsection \<open>Vector Polynomials\<close>
+
+text \<open>We must define the following four constants outside the global interpretation, since otherwise
+  their types are too general.\<close>
+
+definition splus_pprod :: "('a::nat, 'b::nat) pp \<Rightarrow> _"
+  where "splus_pprod = pprod.splus"
+
+definition monom_mult_pprod :: "'c::semiring_0 \<Rightarrow> ('a::nat, 'b::nat) pp \<Rightarrow> _"
+  where "monom_mult_pprod = pprod.monom_mult"
+
+definition mult_scalar_pprod :: "(('a::nat, 'b::nat) pp \<Rightarrow>\<^sub>0 'c::semiring_0) \<Rightarrow> _"
+  where "mult_scalar_pprod = pprod.mult_scalar"
+
+definition adds_term_pprod :: "(('a::nat, 'b::nat) pp \<times> _) \<Rightarrow> _"
+  where "adds_term_pprod = pprod.adds_term"
+
+global_interpretation pprod': gd_nat_term "\<lambda>x::('a, 'b) pp \<times> 'c. x" "\<lambda>x. x" cmp_term
+  rewrites "pprod.pp_of_term = fst"
+  and "pprod.component_of_term = snd"
+  and "pprod.splus = splus_pprod"
+  and "pprod.monom_mult = monom_mult_pprod"
+  and "pprod.mult_scalar = mult_scalar_pprod"
+  and "pprod.adds_term = adds_term_pprod"
+  for cmp_term :: "(('a::nat, 'b::nat) pp \<times> 'c::{nat,the_min}) nat_term_order"
+  defines shift_map_keys_pprod = pprod'.shift_map_keys
+  and min_term_pprod = pprod'.min_term
+  and lt_pprod = pprod'.lt
+  and lc_pprod = pprod'.lc
+  and tail_pprod = pprod'.tail
+  and comp_opt_p_pprod = pprod'.comp_opt_p
+  and ord_p_pprod = pprod'.ord_p
+  and ord_strict_p_pprod = pprod'.ord_strict_p
+  and find_adds_pprod = pprod'.find_adds
+  and trd_aux_pprod= pprod'.trd_aux
+  and trd_pprod = pprod'.trd
+  and spoly_pprod = pprod'.spoly
+  and count_const_lt_components_pprod = pprod'.count_const_lt_components
+  and count_rem_components_pprod = pprod'.count_rem_components
+  and const_lt_component_pprod = pprod'.const_lt_component
+  and full_gb_pprod = pprod'.full_gb
+  and keys_to_list_pprod = pprod'.keys_to_list
+  and Keys_to_list_pprod = pprod'.Keys_to_list
+  and add_pairs_single_sorted_pprod = pprod'.add_pairs_single_sorted
+  and add_pairs_pprod = pprod'.add_pairs
+  and canon_pair_order_aux_pprod = pprod'.canon_pair_order_aux
+  and canon_basis_order_pprod = pprod'.canon_basis_order
+  and new_pairs_sorted_pprod = pprod'.new_pairs_sorted
+  and component_crit_pprod = pprod'.component_crit
+  and chain_ncrit_pprod = pprod'.chain_ncrit
+  and chain_ocrit_pprod = pprod'.chain_ocrit
+  and apply_icrit_pprod = pprod'.apply_icrit
+  and apply_ncrit_pprod = pprod'.apply_ncrit
+  and apply_ocrit_pprod = pprod'.apply_ocrit
+  and trdsp_pprod = pprod'.trdsp
+  and gb_sel_pprod = pprod'.gb_sel
+  and gb_red_aux_pprod = pprod'.gb_red_aux
+  and gb_red_pprod = pprod'.gb_red
+  and gb_aux_pprod = pprod'.gb_aux
+  and gb_pprod = pprod'.gb
+  subgoal by (fact gd_nat_term_id)
+  subgoal by (fact pprod_pp_of_term)
+  subgoal by (fact pprod_component_of_term)
+  subgoal by (simp only: splus_pprod_def)
+  subgoal by (simp only: monom_mult_pprod_def)
+  subgoal by (simp only: mult_scalar_pprod_def)
+  subgoal by (simp only: adds_term_pprod_def)
+  done
+
+lemma compute_adds_term_pprod [code]:
+  "adds_term_pprod u v = (snd u = snd v \<and> adds_pp_add_linorder (fst u) (fst v))"
+  by (simp add: adds_term_pprod_def pprod.adds_term_def adds_pp_add_linorder_def)
+
+lemma compute_splus_pprod [code]: "splus_pprod t (s, i) = (t + s, i)"
+  by (simp add: splus_pprod_def pprod.splus_def)
+
+lemma compute_shift_map_keys_pprod [code abstract]:
+  "list_of_oalist_ntm (shift_map_keys_pprod t f xs) = map_raw (\<lambda>(k, v). (splus_pprod t k, f v)) (list_of_oalist_ntm xs)"
+  by (simp add: pprod'.list_of_oalist_shift_keys case_prod_beta')
+
+lemmas [code] = conversep_iff
+
+definition Vec\<^sub>0 :: "nat \<Rightarrow> (('a, nat) pp \<Rightarrow>\<^sub>0 'b) \<Rightarrow> (('a::nat, nat) pp \<times> nat) \<Rightarrow>\<^sub>0 'b::semiring_1" where
+  "Vec\<^sub>0 i p = mult_scalar_pprod p (Poly_Mapping.single (0, i) 1)"
+
+experiment begin interpretation trivariate\<^sub>0_rat .
+
+lemma
+  "ord_p_pprod (POT DRLEX) (Vec\<^sub>0 1 (X\<^sup>2 * Z) + Vec\<^sub>0 0 (2 * Y ^ 3 * Z\<^sup>2)) (Vec\<^sub>0 1 (X\<^sup>2 * Z\<^sup>2 + 2 * Y ^ 3 * Z\<^sup>2))"
+  by eval
+
+lemma
+  "tail_pprod (POT DRLEX) (Vec\<^sub>0 1 (X\<^sup>2 * Z) + Vec\<^sub>0 0 (2 * Y ^ 3 * Z\<^sup>2)) = Vec\<^sub>0 0 (2 * Y ^ 3 * Z\<^sup>2)"
+  by eval
+
+lemma
+  "lt_pprod (POT DRLEX) (Vec\<^sub>0 1 (X\<^sup>2 * Z) + Vec\<^sub>0 0 (2 * Y ^ 3 * Z\<^sup>2)) = (sparse\<^sub>0 [(0, 2), (2, 1)], 1)"
+  by eval
+
+lemma
+  "keys (Vec\<^sub>0 0 (X\<^sup>2 * Z ^ 3) + Vec\<^sub>0 1 (2 * Y ^ 3 * Z\<^sup>2)) =
+    {(sparse\<^sub>0 [(0, 2), (2, 3)], 0), (sparse\<^sub>0 [(1, 3), (2, 2)], 1)}"
+  by eval
+
+lemma
+  "keys (Vec\<^sub>0 0 (X\<^sup>2 * Z ^ 3) + Vec\<^sub>0 2 (2 * Y ^ 3 * Z\<^sup>2)) =
+    {(sparse\<^sub>0 [(0, 2), (2, 3)], 0), (sparse\<^sub>0 [(1, 3), (2, 2)], 2)}"
+  by eval
+
+lemma
+  "Vec\<^sub>0 1 (X\<^sup>2 * Z ^ 7 + 2 * Y ^ 3 * Z\<^sup>2) + Vec\<^sub>0 3 (X\<^sup>2 * Z ^ 4) + Vec\<^sub>0 1 (- 2 * Y ^ 3 * Z\<^sup>2) =
+    Vec\<^sub>0 1 (X\<^sup>2 * Z ^ 7) + Vec\<^sub>0 3 (X\<^sup>2 * Z ^ 4)"
+  by eval
+
+lemma
+  "lookup (Vec\<^sub>0 0 (X\<^sup>2 * Z ^ 7) + Vec\<^sub>0 1 (2 * Y ^ 3 * Z\<^sup>2 + 2)) (sparse\<^sub>0 [(0, 2), (2, 7)], 0) = 1"
+  by eval
+
+lemma
+  "lookup (Vec\<^sub>0 0 (X\<^sup>2 * Z ^ 7) + Vec\<^sub>0 1 (2 * Y ^ 3 * Z\<^sup>2 + 2)) (sparse\<^sub>0 [(0, 2), (2, 7)], 1) = 0"
+  by eval
+
+lemma
+  "Vec\<^sub>0 0 (0 * X^2 * Z^7) + Vec\<^sub>0 1 (0 * Y^3*Z\<^sup>2) = 0"
+  by eval
+
+lemma
+  "monom_mult_pprod 3 (sparse\<^sub>0 [(1, 2::nat)]) (Vec\<^sub>0 0 (X\<^sup>2 * Z) + Vec\<^sub>0 1 (2 * Y ^ 3 * Z\<^sup>2)) =
+    Vec\<^sub>0 0 (3 * Y\<^sup>2 * Z * X\<^sup>2) + Vec\<^sub>0 1 (6 * Y ^ 5 * Z\<^sup>2)"
+  by eval
+
+lemma
+  "trd_pprod DRLEX [Vec\<^sub>0 0 (Y\<^sup>2 * Z + 2 * Y * Z ^ 3)] (Vec\<^sub>0 0 (X\<^sup>2 * Z ^ 4 - 2 * Y ^ 3 * Z ^ 3)) =
+    Vec\<^sub>0 0 (X\<^sup>2 * Z ^ 4 + Y ^ 4 * Z)"
+  by eval
+
+lemma
+  "length (gb_pprod (POT DRLEX)
+    [
+     (Vec\<^sub>0 0 (X\<^sup>2 * Z ^ 4 - 2 * Y ^ 3 * Z\<^sup>2), ()),
+     (Vec\<^sub>0 0 (Y\<^sup>2 * Z + 2 * Z ^ 3), ())
+    ] ()) = 4"
+  by eval
+
+end
 
 end (* theory *)
