OAlist/Algorithm_Schema_Impl.thy
@@ -6,64 +6,33 @@ theory Algorithm_Schema_Impl
   imports "../Groebner_Bases/Algorithm_Schema" MPoly_Type_Class_OAlist
 begin
 
-lemma compute_card_keys [code]: "card_keys (Pm_oalist xs) = length (list_of_oalist xs)"
-  apply (simp only: card_keys_def compute_keys_pm image_set o_def)
+lemma compute_card_keys [code]: "card_keys (MP_oalist xs) = length (fst (list_of_oalist_ntm xs))"
+  apply (simp only: card_keys_def keys_MP_oalist image_set o_def)
   sorry
-
-instantiation natural :: wellorder
-begin
-
-instance sorry
-
-end
-
-instantiation natural :: countable
-begin
-
-instance sorry
-
-end
-
-instantiation natural :: add_wellorder
-begin
-
-instance sorry
-
-end
-
-instantiation natural :: compare
-begin
-
-definition compare_natural :: "natural comparator" where
-  "compare_natural = comparator_of_le"
-
-instance sorry
-
-end
 
 subsection \<open>Generating Cyclic Polynomials\<close>
 
-definition cycl_pp :: "nat \<Rightarrow> nat \<Rightarrow> nat \<Rightarrow> (natural \<Rightarrow>\<^sub>0 natural)"
-  where "cycl_pp n d i = sparse\<^sub>0 (map (\<lambda>k. (natural_of_nat (modulo (k + i) n), 1)) [0..<d])"
+definition cycl_pp :: "nat \<Rightarrow> nat \<Rightarrow> nat \<Rightarrow> (nat, nat) pp"
+  where "cycl_pp n d i = sparse\<^sub>0 (map (\<lambda>k. (modulo (k + i) n, 1)) [0..<d])"
 
-definition cyclic :: "nat \<Rightarrow> ((natural \<Rightarrow>\<^sub>0 natural) \<Rightarrow>\<^sub>0 'a::{zero,one,uminus}) list"
-  where "cyclic n =
+definition cyclic :: "(nat, nat) pp nat_term_order \<Rightarrow> nat \<Rightarrow> ((nat, nat) pp \<Rightarrow>\<^sub>0 'a::{zero,one,uminus}) list"
+  where "cyclic to n =
             (let xs = [0..<n] in
-              (map (\<lambda>d. sparse\<^sub>0 (map (\<lambda>i. (cycl_pp n d i, 1)) xs)) [1..<n]) @ [sparse\<^sub>0 [(cycl_pp n n 0, 1), (0, -1)]]
+              (map (\<lambda>d. distr\<^sub>0 to (map (\<lambda>i. (cycl_pp n d i, 1)) xs)) [1..<n]) @ [distr\<^sub>0 to [(cycl_pp n n 0, 1), (0, -1)]]
             )"
 
 text \<open>\<open>cyclic n\<close> is a system of \<open>n\<close> polynomials in \<open>n\<close> indeterminates, with maximum degree \<open>n\<close>.\<close>
 
 subsection \<open>Generating Katsura Polynomials\<close>
 
-definition Katsura_poly :: "nat \<Rightarrow> nat \<Rightarrow> ((nat \<Rightarrow>\<^sub>0 nat) \<Rightarrow>\<^sub>0 rat)"
-  where "Katsura_poly n i =
-            (\<Sum>j=-(int n)..<(int n) + 1 - i. Var\<^sub>0 (nat (abs j)) * Var\<^sub>0 (nat (abs j + i))) - Var\<^sub>0 i"
+definition Katsura_poly :: "(nat, nat) pp nat_term_order \<Rightarrow> nat \<Rightarrow> nat \<Rightarrow> ((nat, nat) pp \<Rightarrow>\<^sub>0 rat)"
+  where "Katsura_poly to n i =
+            change_ord to ((\<Sum>j=-(int n)..<(int n) + 1 - i. V\<^sub>0 (nat (abs j)) * V\<^sub>0 (nat (abs j + i))) - V\<^sub>0 i)"
 
-definition Katsura :: "nat \<Rightarrow> ((nat \<Rightarrow>\<^sub>0 nat) \<Rightarrow>\<^sub>0 rat) list"
-  where "Katsura n =
+definition Katsura :: "(nat, nat) pp nat_term_order \<Rightarrow> nat \<Rightarrow> ((nat, nat) pp \<Rightarrow>\<^sub>0 rat) list"
+  where "Katsura to n =
           (let xs = [0..<n] in
-            (sparse\<^sub>0 ((sparse\<^sub>0 [(0, 1)], 1) # (map (\<lambda>i. (sparse\<^sub>0 [(Suc i, 1)], 2)) xs) @ [(0, -1)])) # (map (Katsura_poly n) xs)
+            (distr\<^sub>0 to ((sparse\<^sub>0 [(0, 1)], 1) # (map (\<lambda>i. (sparse\<^sub>0 [(Suc i, 1)], 2)) xs) @ [(0, -1)])) # (map (Katsura_poly to n) xs)
           )"
 
 text \<open>\<open>Katsura n\<close> is a system of \<open>n + 1\<close> polynomials in \<open>n + 1\<close> indeterminates, with maximum degree \<open>2\<close>.\<close>
